compiler/backend/clos_numberScript.sml
@@ -56,4 +56,13 @@ val renumber_code_locs_def = tDefine "renumber_code_locs" `
  rw [exp_size_def] >>
  decide_tac);
 
+val renumber_code_locs_ind = theorem"renumber_code_locs_ind";
+
+val renumber_code_locs_length = store_thm("renumber_code_locs_length",
+  ``(∀x y. LENGTH (SND (renumber_code_locs_list x y)) = LENGTH y) ∧
+    (∀(x:num)(y:closLang$exp). T)``,
+    ho_match_mp_tac renumber_code_locs_ind >>
+    simp[renumber_code_locs_def,UNCURRY] >> rw[] >>
+    METIS_TAC[PAIR,FST,SND]);
+
 val _ = export_theory()
